all done

StoreAtomicity.v
@@ -2,7 +2,8 @@ Require Import DataTypes.
 
 Set Implicit Arguments.
 
-Record Resp := { procR: Cache;
+Record Resp := { addrR: Addr;
+                 procR: Cache;
                  idx: Index;
                  datum: Data
                }.
@@ -10,40 +11,38 @@ Record Resp := { procR: Cache;
 Section StoreAtomicity.
   Variable reqFn: Addr -> Cache -> Index -> Req.
 
-  Variable respFn: Addr -> Time -> option Resp.
+  Variable respFn: Time -> option Resp.
 
-  Variable a: Addr.
-
-  Definition noStore t :=
-    match respFn a t with
-      | Some (Build_Resp c' i' d') =>
-          desc (reqFn a c' i') = St -> False
+  Definition noStore a t :=
+    match respFn t with
+      | Some (Build_Resp a' c' i' d') =>
+          a' = a -> desc (reqFn a c' i') = St -> False
       | _ => True
     end.
 
   Record StoreAtomicity :=
     {
       uniqRespLabels:
-        forall t1 t2, match respFn a t1, respFn a t2 with
-                        | Some (Build_Resp c1 i1 _), Some (Build_Resp c2 i2 _) =>
-                          c1 = c2 -> i1 = i2 -> t1 = t2
+        forall t1 t2, match respFn t1, respFn t2 with
+                        | Some (Build_Resp a1 c1 i1 _), Some (Build_Resp a2 c2 i2 _) =>
+                          a1 = a2 -> c1 = c2 -> i1 = i2 -> t1 = t2
                         | _, _ => True
                       end;
 
       localOrdering:
-        forall t1 t2, match respFn a t1, respFn a t2 with
-                        | Some (Build_Resp c1 i1 _), Some (Build_Resp c2 i2 _) =>
-                          c1 = c2 -> i1 > i2 -> t1 > t2
+        forall t1 t2, match respFn t1, respFn t2 with
+                        | Some (Build_Resp a1 c1 i1 _), Some (Build_Resp a2 c2 i2 _) =>
+                          a1 = a2 -> c1 = c2 -> i1 > i2 -> t1 > t2
                         | _, _ => True
                       end;
 
       allPrevious:
-        forall t2, match respFn a t2 with
-                     | Some (Build_Resp c2 i2 _) =>
+        forall t2, match respFn t2 with
+                     | Some (Build_Resp a2 c2 i2 _) =>
                        forall i1, i1 < i2 -> exists t1, t1 < t2 /\
-                                                        match respFn a t1 with
-                                                          | Some (Build_Resp c1 i _) =>
-                                                            c1 = c2 /\ i = i1
+                                                        match respFn t1 with
+                                                          | Some (Build_Resp a1 c1 i _) =>
+                                                            a1 = a2 /\ c1 = c2 /\ i = i1
                                                           | None => False
                                                         end
                      | _ => True
@@ -51,19 +50,19 @@ Section StoreAtomicity.
 
       storeAtomicity:
         forall t,
-          match respFn a t with
-            | Some (Build_Resp c i d) =>
+          match respFn t with
+            | Some (Build_Resp a c i d) =>
               let (descQ, dtQ) := reqFn a c i in
               match descQ with
                 | Ld =>
-                  (d = initData a /\ forall t', t' < t -> noStore t') \/
+                  (d = initData a /\ forall t', t' < t -> noStore a t') \/
                   (exists tm,
                      tm < t /\
-                     match respFn a tm with
-                       | Some (Build_Resp cm im dm) =>
-                         let (descQm, dtQm) := reqFn a cm im in
-                         d = dtQm /\ descQm = St /\
-                         forall t', tm < t' < t -> noStore t'
+                     match respFn tm with
+                       | Some (Build_Resp am cm im dm) =>
+                         let (descQm, dtQm) := reqFn am cm im in
+                         a = am /\ d = dtQm /\ descQm = St /\
+                         forall t', tm < t' < t -> noStore a t'
                        | _ => False
                      end)
                 | St => d = initData zero 
