Top.v
@@ -12,13 +12,12 @@ Module mkTop.
   Module l1T := LatestValueTheorems mkDataTypes ch ba l1 comp lv.
     Import mkDataTypes l1 l1T.
 
-
-    Definition respFn a t :=
-      match deqOrNot a t with
+    Definition respFn t :=
+      match deqOrNot t with
         | inleft pf =>
           match pf with
-            | exist (c,i) _ =>
-              Some (Build_Resp c i
+            | exist (a, c,i) _ =>
+              Some (Build_Resp a c i
                                match desc (reqFn a c i) with
                                  | Ld => data c a t
                                  | St => initData zero
@@ -33,33 +32,33 @@ Module mkTop.
                           end; simpl in *.
 
     Theorem uniqRespLabels':
-      forall {a t1 t2}, match respFn a t1, respFn a t2 with
-                        | Some (Build_Resp c1 i1 _), Some (Build_Resp c2 i2 _) =>
-                          c1 = c2 -> i1 = i2 -> t1 = t2
+      forall {t1 t2}, match respFn t1, respFn t2 with
+                        | Some (Build_Resp a1 c1 i1 _), Some (Build_Resp a2 c2 i2 _) =>
+                          a1 = a2 -> c1 = c2 -> i1 = i2 -> t1 = t2
                         | _, _ => True
                       end.
     Proof.
-      intros a t1 t2; unfold respFn;
-      destruct (deqOrNot a t1); destruct (deqOrNot a t2);
-      solve [finish; intros H H0; rewrite <- H in *; rewrite <- H0 in *;
+      intros t1 t2; unfold respFn;
+      destruct (deqOrNot t1); destruct (deqOrNot t2);
+      solve [finish; intros H H0 H1; rewrite <- H, <- H1 in *; rewrite <- H0 in *;
              apply (uniqDeqProc2 d0 d) |
              finish; intuition | 
              intuition].
     Qed.
 
     Theorem localOrdering':
-      forall {a t1 t2}, match respFn a t1, respFn a t2 with
-                        | Some (Build_Resp c1 i1 _), Some (Build_Resp c2 i2 _) =>
-                          c1 = c2 -> i1 > i2 -> t1 > t2
+      forall {t1 t2}, match respFn t1, respFn t2 with
+                        | Some (Build_Resp a1 c1 i1 _), Some (Build_Resp a2 c2 i2 _) =>
+                          a1 = a2 -> c1 = c2 -> i1 > i2 -> t1 > t2
                         | _, _ => True
                       end.
     Proof.
-      intros a t1 t2; unfold respFn;
-      destruct (deqOrNot a t1); destruct (deqOrNot a t2).
+      intros t1 t2; unfold respFn;
+      destruct (deqOrNot t1); destruct (deqOrNot t2).
       finish.
-      intros H H0.
-      rewrite H in *.
-      pose proof (deqOrder d d0 H0).
+      intros H H0 H1.
+      rewrite H, H0 in *.
+      pose proof (deqOrder d d0 H1).
       unfold Time in *.
       assert (opts: t1 = t2 \/ t1 > t2) by omega.
       destruct opts as [e1 | e2].
@@ -73,48 +72,48 @@ Module mkTop.
     Qed.
 
     Theorem allPrevious':
-      forall {a t2}, match respFn a t2 with
-                     | Some (Build_Resp c2 i2 _) =>
+      forall {t2}, match respFn t2 with
+                     | Some (Build_Resp a2 c2 i2 _) =>
                        forall {i1}, i1 < i2 -> exists t1, t1 < t2 /\
-                                                          match respFn a t1 with
-                                                            | Some (Build_Resp c1 i _) =>
-                                                              c1 = c2 /\ i = i1
+                                                          match respFn t1 with
+                                                            | Some (Build_Resp a1 c1 i _) =>
+                                                              a1 = a2 /\ c1 = c2 /\ i = i1
                                                             | None => False
                                                           end
                      | _ => True
                    end.
     Proof.
-      intros a t2; unfold respFn.
-      destruct (deqOrNot a t2).
+      intros t2; unfold respFn.
+      destruct (deqOrNot t2).
       finish.
       intros i1 cond.
       pose proof (deqImpDeqBefore d cond) as [t' [cond2 deq2]].
       exists t'.
-      destruct (deqOrNot a t').
+      destruct (deqOrNot t').
       finish.
       constructor.
       intuition.
       apply (uniqDeqProc3 d0 deq2).
       constructor.
       intuition.
-      apply (n _ _ deq2).
+      apply (n _ _ _ deq2).
       intuition.
     Qed.
 
     Theorem storeAtomicity':
-        forall a t,
-          match respFn a t with
-            | Some (Build_Resp c i d) =>
+        forall t,
+          match respFn t with
+            | Some (Build_Resp a c i d) =>
               let (descQ, dtQ) := reqFn a c i in
               match descQ with
                 | Ld =>
                   (d = initData a /\ forall t', t' < t -> noStore reqFn respFn a t') \/
                   (exists tm,
                      tm < t /\
-                     match respFn a tm with
-                       | Some (Build_Resp cm im dm) =>
-                         let (descQm, dtQm) := reqFn a cm im in
-                         d = dtQm /\ descQm = St /\
+                     match respFn tm with
+                       | Some (Build_Resp am cm im dm) =>
+                         let (descQm, dtQm) := reqFn am cm im in
+                         a = am /\ d = dtQm /\ descQm = St /\
                          forall t', tm < t' < t -> noStore reqFn respFn a t'
                        | _ => False
                      end)
@@ -123,10 +122,10 @@ Module mkTop.
             | _ => True
           end.
     Proof.
-      intros a t.
+      intros t.
       unfold respFn.
       unfold noStore.
-      destruct (deqOrNot a t).
+      destruct (deqOrNot t).
       finish.
       pose proof (processDeq d) as procD.
       destruct (reqFn a c i); simpl.
@@ -140,13 +139,14 @@ Module mkTop.
       destruct lv as [[dtMatch noPrev]|prev].
       left.
       constructor; intuition.
-      destruct (deqOrNot a t').
+      destruct (deqOrNot t').
       finish.
       pose proof (deqDef d0) as def0.
       assert (cond: 0 <= t' < t) by omega.
       specialize (noPrev _ cond _ i0 def0).
       destruct (reqFn a c0 i0).
       intros; simpl in *.
+      rewrite H0 in *.
       intuition.
       intuition.
       right.
@@ -154,16 +154,19 @@ Module mkTop.
       exists tb.
       constructor.
       intuition.
-      destruct (deqOrNot a tb).
+      destruct (deqOrNot tb).
       finish.
-      pose proof (uniqDeqProc3 deq_tb d0) as [ceq ieq].
-      rewrite <- ceq in *; rewrite <- ieq in *.
+      pose proof (uniqDeqProc3 deq_tb d0) as [aeq [ceq ieq]].
+      rewrite <- ceq in *; rewrite <- ieq, <- aeq in *.
       destruct (reqFn a cb ib); simpl in *.
       constructor. intuition.
       constructor. intuition.
+      constructor. intuition.
       intros t' cond.
-      destruct (deqOrNot a t').
+      destruct (deqOrNot t').
       finish.
+      intros x.
+      rewrite x in *.
       pose proof (deqDef d1) as defdeq.
       specialize (rest _ cond _ i1 defdeq).
       destruct (reqFn a c1 i1); simpl in *.
@@ -171,7 +174,7 @@ Module mkTop.
 
       intuition.
 
-      apply (n _ _ deq_tb).
+      apply (n _ _ _ deq_tb).
       intuition.
       intuition.
     Qed.
@@ -179,9 +182,9 @@ Module mkTop.
     About StoreAtomicity.
 
 
-    Theorem sa a: StoreAtomicity reqFn respFn a.
+    Theorem sa: StoreAtomicity reqFn respFn.
     Proof.
-      apply (Build_StoreAtomicity reqFn respFn a
-            (@uniqRespLabels' a) (@localOrdering' a) (@allPrevious' a) (storeAtomicity' a)).
+      apply (Build_StoreAtomicity reqFn respFn
+            (@uniqRespLabels') (@localOrdering') (@allPrevious') (storeAtomicity')).
     Qed.
 End mkTop.
